

## Q1 - 24 January - Shift 1

$\lim_{t \rightarrow 0} \left( 1^{\frac{1}{\sin^2 t}} + 2^{\frac{1}{\sin^2 t}} + \dots + n^{\frac{1}{\sin^2 t}} \right)^{\sin^2 t}$  is equal to

(1)  $n^2 + n$

(2)  $n$

(3)  $\frac{n(n+1)}{2}$

(4)  $n^2$

Space for your notes:

## Q2 - 24 January - Shift 2

The set of all values of  $a$  for which  $\lim_{x \rightarrow a} ([x - 5] - [2x + 2]) = 0$ , where  $[\infty]$  denotes the greater integer less than or equal to  $\infty$  is equal to

(1)  $(-7.5, -6.5)$

(2)  $(-7.5, -6.5]$

(3)  $[-7.5, -6.5]$

(4)  $[-7.5, -6.5)$

Space for your notes:

## Q3 - 29 January - Shift 1

Let  $x = 2$  be a root of the equation  $x^2 + px + q = 0$

$$\text{and } f(x) = \begin{cases} \frac{1 - \cos(x^2 - 4px + q^2 + 8q + 16)}{(x - 2p)^4}, & x \neq 2p \\ 0, & x = 2p \end{cases}$$

Then  $\lim_{x \rightarrow 2p^+} [f(x)]$

where  $[.]$  denotes greatest integer function, is

(1) 2

(2) 1

(3) 0

(4) -1

Space for your notes:

## Q4 - 30 January - Shift 2

Let  $f$ ,  $g$  and  $h$  be the real valued functions defined

$$\text{on } \mathbb{R} \text{ as } f(x) = \begin{cases} \frac{x}{|x|}, & x \neq 0 \\ 1, & x = 0 \end{cases},$$

$$g(x) = \begin{cases} \frac{\sin(x+1)}{(x+1)}, & x \neq -1 \\ 1, & x = -1 \end{cases} \text{ and } h(x) = 2[x] - f(x),$$

where  $[x]$  is the greatest integer  $\leq x$ . Then the

value of  $\lim_{x \rightarrow 1} g(h(x-1))$  is

- (1) 1
- (2)  $\sin(1)$
- (3) -1
- (4) 0

Space for your notes:

#### Q5 - 31 January - Shift 2

$$\text{Hence } y \in \left(-\infty, -\frac{21}{4}\right] \cup [0, \infty)$$

$$\lim_{x \rightarrow \infty} \frac{\left(\sqrt{3x+1} + \sqrt{3x-1}\right)^6 + \left(\sqrt{3x+1} - \sqrt{3x-1}\right)^6}{\left(x + \sqrt{x^2-1}\right)^6 + \left(x - \sqrt{x^2-1}\right)^6} x^3$$

- (1) is equal to 9
- (2) is equal to 27
- (3) does not exist
- (4) is equal to  $\frac{27}{2}$

Space for your notes:

// mathongo // mathongo // mathongo // mathongo // mathongo // mathongo

Answer Key

// mathongo // mathongo // mathongo // mathongo // mathongo // mathongo

(As per Official NTA Key released on 2 Feb)

// mathongo // mathongo // mathongo // mathongo // mathongo // mathongo

Q1 (2)

Q2 (1)

Q3 (3)

Q4 (1)

// mathongo // mathongo // mathongo // mathongo // mathongo // mathongo

Q5 (2)

// mathongo // mathongo // mathongo // mathongo // mathongo // mathongo

// mathongo // mathongo // mathongo // mathongo // mathongo // mathongo

// mathongo // mathongo // mathongo // mathongo // mathongo // mathongo

// mathongo // mathongo // mathongo // mathongo // mathongo // mathongo

// mathongo // mathongo // mathongo // mathongo // mathongo // mathongo

// mathongo // mathongo // mathongo // mathongo // mathongo // mathongo

// mathongo // mathongo // mathongo // mathongo // mathongo // mathongo

// mathongo // mathongo // mathongo // mathongo // mathongo // mathongo

// mathongo // mathongo // mathongo // mathongo // mathongo // mathongo

// mathongo // mathongo // mathongo // mathongo // mathongo // mathongo

// mathongo // mathongo // mathongo // mathongo // mathongo // mathongo

// mathongo // mathongo // mathongo // mathongo // mathongo // mathongo

// mathongo // mathongo // mathongo // mathongo // mathongo // mathongo

// mathongo // mathongo // mathongo // mathongo // mathongo // mathongo

// mathongo // mathongo // mathongo // mathongo // mathongo // mathongo

// mathongo // mathongo // mathongo // mathongo // mathongo // mathongo

// mathongo // mathongo // mathongo // mathongo // mathongo // mathongo

#MathBoleTohMathonGo

Q1 (2)

$$\lim_{t \rightarrow 0} \left( 1^{\operatorname{cosec}^2 t} + 2^{\operatorname{cosec}^2 t} + \dots + n^{\operatorname{cosec}^2 t} \right)^{\sin^2 t}$$

$$= \lim_{t \rightarrow 0} n^{\left( \left( \frac{1}{n} \right)^{\operatorname{cosec}^2 t} + \left( \frac{2}{n} \right)^{\operatorname{cosec}^2 t} + \dots + 1 \right)^{\sin^2 t}}$$

$$= n$$

Q2 (1)

#MathBoleTohMathonGo

$$\lim_{x \rightarrow a} ([x - 5] - [2x + 2]) = 0$$

$$\lim_{x \rightarrow a} ([x] - 5 - [2x] - 2) = 0$$

$$\lim_{x \rightarrow a} ([x] - [2x]) = 7$$

$$[a] - [2a] = 7$$

$$a \in I, \quad a = -7$$

$$a \notin I, \quad a = I + f$$

$$\text{Now, } [a] - [2a] = 7$$

$$-I - [2f] = 7$$

$$\text{Case-I: } f \in \left(0, \frac{1}{2}\right)$$

$$2f \in (0, 1)$$

$$-I = 7$$

$$I = -7 \Rightarrow a \in (-7, -6.5)$$

$$\text{Case-II: } f \in \left(\frac{1}{2}, 1\right)$$

$$2f \in (1, 2)$$

$$-I - 1 = 7$$

$$I = -8 \Rightarrow a \in (-7.5, -7)$$

$$\text{Hence, } a \in (-7.5, -6.5)$$

#MathBoleTohMathonGo

**Q3 (3)**

$$\lim_{x \rightarrow 2p^+} \left( \frac{1 - \cos(x^2 - 4px + q^2 + 8q + 16)}{(x^2 - 4px + q^2 + 8q + 16)^2} \right) \left( \frac{(x^2 - 4px + q^2 + 8q + 16)^2}{(x - 2p)^2} \right)$$

$$\lim_{h \rightarrow 0} \frac{1}{2} \left( \frac{(2p + h)^2 - 4p(2p + h) + q^2 + 8q + 16}{h^2} \right)^2 = \frac{1}{2}$$

Using L'Hospital's

$$\lim_{x \rightarrow 2p^+} [f(x)] = 0$$

**Q4 (1)**

$$\text{LHL} = \lim_{k \rightarrow 0} g(h(-k)), k > 0$$

$$= \lim_{k \rightarrow 0} g(-2 + 1) \because f(x) = -1 \forall x < 0$$

$$= g(-1) = 1$$

$$\text{RHL} = \lim_{k \rightarrow 0} g(h(k)), k > 0$$

$$= \lim_{k \rightarrow 0} g(-1) \because f(x) = 1, \forall x > 0$$

$$= 1$$

**Q5 (2)**

#MathBoleTohMathonGo



$$\lim_{x \rightarrow \infty} \frac{(\sqrt{3x+1} + \sqrt{3x-1})^6 + (\sqrt{3x+1} - \sqrt{3x-1})^6}{(x + \sqrt{x^2-1})^6 + (x - \sqrt{x^2-1})^6} x^3$$

$$\lim_{x \rightarrow \infty} x^3 \times \left\{ \frac{x^3 \left\{ \left( \sqrt{3 + \frac{1}{x}} + \sqrt{3 - \frac{1}{x}} \right)^6 + \left( \sqrt{3 + \frac{1}{x}} - \sqrt{3 - \frac{1}{x}} \right)^6 \right\}}{x^6 \left\{ \left( 1 + \sqrt{1 - \frac{1}{x^2}} \right)^6 + \left( 1 - \sqrt{1 - \frac{1}{x^2}} \right)^6 \right\}} \right\}$$

$$= \frac{(2\sqrt{3})^6 + 0}{2^6 + 0} = 3^3 = (27)$$